some more work on alpha equivalence

Transformations/Alpha_Equiv.thy
@@ -68,25 +68,26 @@ definition get_fun_decls ::
   (case get_fun_decls' l 0 of
     (l', _) \<Rightarrow> l')"
 
-
+(* we split into function and variable namespaces
+ * since that is how the interpreter works *)
 fun alpha_equiv_expr' ::
-  "subst \<Rightarrow> ('v, 't) YulExpression \<Rightarrow> ('v, 't) YulExpression \<Rightarrow> bool" where
-  "alpha_equiv_expr' scopes
+  "subst \<Rightarrow> subst \<Rightarrow> ('v, 't) YulExpression \<Rightarrow> ('v, 't) YulExpression \<Rightarrow> bool" where
+  "alpha_equiv_expr' vsubst fsubst
     (YulLiteralExpression x1) (YulLiteralExpression x2) = (x1 = x2)"
-| "alpha_equiv_expr' scopes
+| "alpha_equiv_expr' vsubst fsubst
     (YulIdentifier x1) (YulIdentifier x2) =
-    (subst_lookup scopes x1 = Some x2)"
+    (subst_lookup vsubst x1 = Some x2)"
 (* TODO: we may need to either put a stronger predicate on subst,
  * or have these checks go "both ways" *)
-| "alpha_equiv_expr' scopes
+| "alpha_equiv_expr' vsubst fsubst
     (YulFunctionCallExpression (YulFunctionCall fn1 args1))
     (YulFunctionCallExpression (YulFunctionCall fn2 args2)) =
-    (subst_lookup scopes fn1 = Some fn2 \<and>
-    (list_all2 (alpha_equiv_expr' scopes) args1 args2))"
-| "alpha_equiv_expr' scopes _ _ = False"
+    (subst_lookup fsubst fn1 = Some fn2 \<and>
+    (list_all2 (alpha_equiv_expr' vsubst fsubst) args1 args2))"
+| "alpha_equiv_expr' scopes _ _ _ = False"
 
-definition alpha_equiv_name :: "subst \<Rightarrow> YulIdentifier \<Rightarrow> YulIdentifier \<Rightarrow> bool" where
-"alpha_equiv_name scopes n1 n2 =
+definition alpha_equiv_name' :: "subst \<Rightarrow> YulIdentifier \<Rightarrow> YulIdentifier \<Rightarrow> bool" where
+"alpha_equiv_name' scopes n1 n2 =
   (subst_lookup scopes n1 = Some n2)"
 
 definition alpha_equiv_typed_name' ::
@@ -99,7 +100,8 @@ definition alpha_equiv_typed_name' ::
       | Some n2 \<Rightarrow> tn2 = YulTypedName n2 t1))"
 
 definition alpha_equiv_check_decls ::
-  "('v, 't) YulStatement list \<Rightarrow> ('v, 't) YulStatement list \<Rightarrow> (YulIdentifier * YulIdentifier) list option"
+  "('v, 't) YulStatement list \<Rightarrow> ('v, 't) YulStatement list \<Rightarrow>
+    ((YulIdentifier * YulIdentifier) list * (YulIdentifier * YulIdentifier) list) option"
   where
 "alpha_equiv_check_decls body1 body2 =
   (let vdecls1 = get_var_decls body1 in
@@ -107,40 +109,40 @@ definition alpha_equiv_check_decls ::
   (let vdecls2 = get_var_decls body2 in
   (let fdecls2 = get_fun_decls body2 in
   (if (length vdecls1 = length vdecls2 \<and> length fdecls1 = length fdecls2)
-   then Some (zip (vdecls1 @ fdecls1) (vdecls2 @ fdecls2))
+   then Some (zip vdecls1 vdecls2, zip fdecls1 fdecls2)
    else None)))))"
   
 
 fun alpha_equiv_statement' ::
-  "subst \<Rightarrow> ('v, 't) YulStatement \<Rightarrow> ('v, 't) YulStatement \<Rightarrow> bool" where
-  "alpha_equiv_statement' scopes
+  "subst \<Rightarrow> subst \<Rightarrow> ('v, 't) YulStatement \<Rightarrow> ('v, 't) YulStatement \<Rightarrow> bool" where
+  "alpha_equiv_statement' vsubst fsubst
     (YulFunctionCallStatement (YulFunctionCall fn1 args1)) stm2 =
     (case stm2 of
       (YulFunctionCallStatement (YulFunctionCall fn2 args2)) \<Rightarrow>
-        (subst_lookup scopes fn1 = Some fn2 \<and>
-        (list_all2 (alpha_equiv_expr' scopes) args1 args2))
+        (subst_lookup fsubst fn1 = Some fn2 \<and>
+        (list_all2 (alpha_equiv_expr' vsubst fsubst) args1 args2))
       | _ \<Rightarrow> False)"
 
-| "alpha_equiv_statement' scopes
+| "alpha_equiv_statement' vsubst fsubst
     (YulAssignmentStatement (YulAssignment ns1 e1)) stm2 =
     (case stm2 of
       (YulAssignmentStatement (YulAssignment ns2 e2)) \<Rightarrow>
-        (alpha_equiv_expr' scopes e1 e2 \<and>
-         those (map (subst_lookup scopes) ns1) = Some ns2)
+        (alpha_equiv_expr' vsubst fsubst e1 e2 \<and>
+         those (map (subst_lookup vsubst) ns1) = Some ns2)
       | _ \<Rightarrow> False)"
 
-| "alpha_equiv_statement' scopes
+| "alpha_equiv_statement' vsubst fsubst
     (YulVariableDeclarationStatement (YulVariableDeclaration ns1 eo1)) stm2 =
     (case stm2 of
       (YulVariableDeclarationStatement (YulVariableDeclaration ns2 eo2)) \<Rightarrow>
         ((case (eo1, eo2) of
-          (Some e1, Some e2) \<Rightarrow> alpha_equiv_expr' scopes e1 e2
+          (Some e1, Some e2) \<Rightarrow> alpha_equiv_expr' vsubst fsubst e1 e2
           | (None, None) \<Rightarrow> True
           | _ \<Rightarrow> False) \<and>
          (length ns1 = length ns2))
       | _ \<Rightarrow> False)"
 
-| "alpha_equiv_statement' scopes
+| "alpha_equiv_statement' vsubst fsubst
   (YulFunctionDefinitionStatement
       (YulFunctionDefinition name1 args1 rets1 body1)) stm2 =
   (case stm2 of
@@ -148,7 +150,7 @@ fun alpha_equiv_statement' ::
         (YulFunctionDefinition name2 args2 rets2 body2)) \<Rightarrow>
         (case alpha_equiv_check_decls body1 body2 of
           None \<Rightarrow> False
-          | Some scopes' \<Rightarrow>
+          | Some (vsubst', fsubst') \<Rightarrow>
             (length args1 = length args2 \<and>
              length rets1 = length rets2 \<and>
              (let newscope1 =
@@ -157,26 +159,28 @@ fun alpha_equiv_statement' ::
              (let newscope2 =
                 ((map (\<lambda> x . case x of (YulTypedName n t) \<Rightarrow> n) args2) @
                  (map (\<lambda> x . case x of (YulTypedName n t) \<Rightarrow> n) rets2)) in
-             (list_all2 (alpha_equiv_statement' (((zip newscope1 newscope2) @ scopes') # scopes))
+             (list_all2 (alpha_equiv_statement' 
+              (((zip newscope1 newscope2) @ vsubst') # vsubst)
+              (fsubst' # fsubst))
               body1 body2)))))
       | _ \<Rightarrow> False)"
 
-| "alpha_equiv_statement' scopes
+| "alpha_equiv_statement' vsubst fsubst
   (YulIf e1 body1) stm2 =
   (case stm2 of
     (YulIf e2 body2) \<Rightarrow>
-      (alpha_equiv_expr' scopes e1 e2 \<and>
+      (alpha_equiv_expr' vsubst fsubst e1 e2 \<and>
       (case alpha_equiv_check_decls body1 body2 of
         None \<Rightarrow> False
-        | Some scopes' \<Rightarrow>
-          list_all2 (alpha_equiv_statement' (scopes' # scopes)) body1 body2))
+        | Some (vsubst', fsubst') \<Rightarrow>
+          list_all2 (alpha_equiv_statement' (vsubst' # vsubst) (fsubst' # fsubst)) body1 body2))
     | _ \<Rightarrow> False)"
-
-| "alpha_equiv_statement' scopes
+  
+| "alpha_equiv_statement' vsubst fsubst
   (YulSwitch e1 cases1) stm2 =
   (case stm2 of
     (YulSwitch e2 cases2) \<Rightarrow>
-      (alpha_equiv_expr' scopes e1 e2 \<and>
+      (alpha_equiv_expr' vsubst fsubst e1 e2 \<and>
       (list_all2
         (\<lambda> c1 c2 .
           (case c1 of
@@ -186,135 +190,167 @@ fun alpha_equiv_statement' ::
             (l1 = l2 \<and>
             (case alpha_equiv_check_decls body1 body2 of
               None \<Rightarrow> False
-              | Some scopes' \<Rightarrow>
-                list_all2 (alpha_equiv_statement' (scopes' # scopes)) body1 body2)))))
+              | Some (vsubst', fsubst') \<Rightarrow>
+                list_all2 (alpha_equiv_statement' (vsubst' # vsubst) (fsubst' # fsubst)) body1 body2)))))
         cases1 cases2))
     | _ \<Rightarrow> False)"
 
-| "alpha_equiv_statement' scopes
+| "alpha_equiv_statement' vsubst fsubst
   (YulForLoop pre1 cond1 post1 body1) stm2 =
   (case stm2 of
     (YulForLoop pre2 cond2 post2 body2) \<Rightarrow>
       (case alpha_equiv_check_decls pre1 pre2 of
         None \<Rightarrow> False
-        | Some scopes'_pre \<Rightarrow> 
+        | Some (vsubst'_pre, fsubst'_pre) \<Rightarrow> 
       (case alpha_equiv_check_decls post1 post2 of
         None \<Rightarrow> False
-        | Some scopes'_post \<Rightarrow>
+        | Some (vsubst'_post, fsubst'_post) \<Rightarrow>
       (case alpha_equiv_check_decls body1 body2 of
         None \<Rightarrow> False
-        | Some scopes'_body \<Rightarrow>
-          (alpha_equiv_expr' (scopes'_pre # scopes) cond1 cond2 \<and>
-           list_all2 (alpha_equiv_statement' (scopes'_pre # scopes)) pre1 pre2 \<and>
-           list_all2 (alpha_equiv_statement' ((scopes'_pre @ scopes'_body) # scopes)) body1 body2 \<and>
-           list_all2 (alpha_equiv_statement' ((scopes'_pre @ scopes'_post) # scopes)) post1 post2))))
+        | Some (vsubst'_body, fsubst'_body) \<Rightarrow>
+          (alpha_equiv_expr' (vsubst'_pre # vsubst) (fsubst'_pre # fsubst) cond1 cond2 \<and>
+           list_all2 (alpha_equiv_statement' (vsubst'_pre # vsubst) (fsubst'_pre # fsubst)) pre1 pre2 \<and>
+           list_all2 (alpha_equiv_statement' ((vsubst'_body @ vsubst'_pre) # vsubst)
+                                             ((fsubst'_body @ fsubst'_pre) # fsubst)) body1 body2 \<and>
+           list_all2 (alpha_equiv_statement' ((vsubst'_post @ vsubst'_pre) # vsubst)
+                                             ((fsubst'_post @ fsubst'_pre) # fsubst)) post1 post2))))
     | _ \<Rightarrow> False)"
 
-| "alpha_equiv_statement' scopes
+| "alpha_equiv_statement' vsubst fsubst
   YulBreak stm2 =
   (case stm2 of
     YulBreak \<Rightarrow> True
     | _ \<Rightarrow> False)"
 
-| "alpha_equiv_statement' scopes
+| "alpha_equiv_statement' vsubst fsubst
   YulContinue stm2 =
   (case stm2 of
     YulContinue \<Rightarrow> True
     | _ \<Rightarrow> False)"
 
-| "alpha_equiv_statement' scopes
+| "alpha_equiv_statement' vsubst fsubst
   YulLeave stm2 =
   (case stm2 of
     YulLeave \<Rightarrow> True
     | _ \<Rightarrow> False)"
 
-| "alpha_equiv_statement' scopes
+| "alpha_equiv_statement' vsubst fsubst
   (YulBlock body1) stm2 =
   (case stm2 of
     (YulBlock body2) \<Rightarrow>
       (case alpha_equiv_check_decls body1 body2 of
         None \<Rightarrow> False
-        | Some scopes' \<Rightarrow> list_all2 (alpha_equiv_statement' (scopes' # scopes)) body1 body2)
+        | Some (vsubst', fsubst') \<Rightarrow>
+          list_all2 (alpha_equiv_statement' (vsubst' # vsubst) (fsubst' # fsubst)) body1 body2)
     | _ \<Rightarrow> False)"
 
-fun alpha_equiv_locals' ::
-  "subst \<Rightarrow> 'v locals \<Rightarrow> 'v locals \<Rightarrow> bool" where
-"alpha_equiv_locals' subst [] [] = True"
-| "alpha_equiv_locals' subst ((n1, v1)#t1) ((n2, v2)#t2) =
-   (v1 = v2 \<and>
-    subst_lookup subst n1 = Some n2 \<and>
-    alpha_equiv_locals' subst t1 t2)"
-| "alpha_equiv_locals' _ _ _ = False"
+term "undefined :: 'v locals"
 
-(* Not yet finished - remaining primitives from Renamer_DeBruijn_Ext_Correct *)
+definition alpha_equiv_local ::
+  "subst \<Rightarrow> subst \<Rightarrow> (YulIdentifier * 'v) \<Rightarrow> (YulIdentifier * 'v) \<Rightarrow> bool" where
+"alpha_equiv_local vsubst fsubst loc1 loc2 =
+  (case loc1 of (n1, v1) \<Rightarrow>
+  (case loc2 of (n2, v2) \<Rightarrow>
+  (v1 = v2 \<and> subst_lookup vsubst n1 = Some n2)))"
+
+definition alpha_equiv_locals' ::
+  "subst \<Rightarrow> subst \<Rightarrow> (YulIdentifier * 'v) list \<Rightarrow> (YulIdentifier * 'v) list \<Rightarrow> bool" where
+"alpha_equiv_locals' vsubst fsubst locs1 locs2 =
+  list_all2 (alpha_equiv_local vsubst fsubst) locs1 locs2"
 
 (*
+definition alpha_equiv_locals' ::
+  "subst \<Rightarrow> subst \<Rightarrow> 'v locals \<Rightarrow> 'v locals \<Rightarrow> bool" where
+"alpha_equiv_locals' vsubst fsubst [] [] = True"
+| "alpha_equiv_locals' vsubst fsubst ((n1, v1)#t1) ((n2, v2)#t2) =
+   (v1 = v2 \<and>
+    subst_lookup vsubst n1 = Some n2 \<and>
+    alpha_equiv_locals' vsubst fsubst t1 t2)"
+| "alpha_equiv_locals' _ _ _ _ = False"
+*)
+
+(* TODO: need equality of function parameters/returns here?
+ * or just alpha equivalence?
+ * i think alpha equivalence should suffice. but under what context?
+ *)
+(* builtins need to be exactly equal.
+ * TODO: perhaps revisit
+ * TODO: can we get away with something weaker than alpha_equiv_statement' here?
+ *  *)
 definition alpha_equiv_function_sig'_scheme ::
-  "subst \<Rightarrow> YulIdentifier \<Rightarrow> ('g, 'v, 't, 'z) function_sig'_scheme \<Rightarrow> YulIdentifier \<Rightarrow> ('g, 'v, 't, 'z) function_sig'_scheme \<Rightarrow> bool" where
-"alpha_equiv_function_sig'_scheme subst n1 s1 n2 s2 =
-  (subst1 subst n1 = Some n2 \<and>
+  "subst \<Rightarrow> subst \<Rightarrow> YulIdentifier \<Rightarrow> ('g, 'v, 't, 'z) function_sig'_scheme \<Rightarrow> YulIdentifier \<Rightarrow> ('g, 'v, 't, 'z) function_sig'_scheme \<Rightarrow> bool" where
+"alpha_equiv_function_sig'_scheme vsubst fsubst n1 s1 n2 s2 =
   (case (f_sig_body s1, f_sig_body s2) of
-        (YulBuiltin b1, YulBuiltin b2) \<Rightarrow>
-          (let args1 = (map (\<lambda> x . case x of (YulTypedName n t) \<Rightarrow> n) (f_sig_arguments s1)) in
-          (let args2 = (map (\<lambda> x . case x of (YulTypedName n t) \<Rightarrow> n) (f_sig_arguments s2)) in
-          (let rets1 = (map (\<lambda> x . case x of (YulTypedName n t) \<Rightarrow> n) (f_sig_returns s1)) in
-          (let rets2 = (map (\<lambda> x . case x of (YulTypedName n t) \<Rightarrow> n) (f_sig_returns s2)) in
-            ((subst_list subst args1 = Some args2) \<and> (subst_list subst rets1 = Some rets2))))))
+        (YulBuiltin b1, YulBuiltin b2) \<Rightarrow> s1 = s2
         | (YulFunction sts1, YulFunction sts2) \<Rightarrow>
-            alpha_equiv_statement' subst 
+          alpha_equiv_statement' vsubst fsubst
               (YulFunctionDefinitionStatement (YulFunctionDefinition n1 (f_sig_arguments s1) (f_sig_returns s1) sts1))
               (YulFunctionDefinitionStatement (YulFunctionDefinition n2 (f_sig_arguments s2) (f_sig_returns s2) sts2))
-        | (_, _) \<Rightarrow> False))"
+        | (_, _) \<Rightarrow> False)"
 
-(* alpha_equiv_function_sig - compare visible ids *)
-definition alpha_equiv_function_sig' ::
-  "subst \<Rightarrow> YulIdentifier \<Rightarrow> ('g, 'v, 't) function_sig \<Rightarrow> YulIdentifier \<Rightarrow> ('g, 'v, 't) function_sig \<Rightarrow> bool" where
-"alpha_equiv_function_sig' subst n1 s1 n2 s2 =
-  (subst_list subst (f_sig_visible s1) = Some (f_sig_visible s2) \<and>
-   alpha_equiv_function_sig'_scheme subst n1 s1 n2 s2)"
-
+(* alpha_equiv_function_sig. TODO: do we need to compare visible ids, or can we get away
+ * with not doing so? *)
 (*
-fun alpha_equiv_function_bodies' ::
-  "subst \<Rightarrow> ('g, 'v, 't) YulFunctionBody \<Rightarrow> ('g, 'v, 't) YulFunctionBody \<Rightarrow> bool" where
-"alpha_equiv_function_bodies subst (YulBuiltin f1) (YulBuiltin f2) = (f1 = f2)"
-| "alpha_equiv_function_bodies subst (YulFunction sts1) (YulFunction sts2) =
-    alpha_equiv_statement' subst
-      (YulFunctionDefinitionStatement (YulFunctionDefinition n1 (f_sig_arguments s1) (f_sig_returns s1) (f_sig_body s1)))
-      (YulFunctionDefinitionStatement (YulFunctionDefinition n2 (f_sig_arguments s2) (f_sig_returns s2) (f_sig_body s2)))"
+definition alpha_equiv_function_sig' ::
+  "subst \<Rightarrow> subst \<Rightarrow> YulIdentifier \<Rightarrow> ('g, 'v, 't) function_sig \<Rightarrow> YulIdentifier \<Rightarrow> ('g, 'v, 't) function_sig \<Rightarrow> bool" where
+"alpha_equiv_function_sig' vsubst fsubst n1 s1 n2 s2 =
+  (those (map (subst_lookup fsubst) (f_sig_visible s1)) = Some (f_sig_visible s2) \<and>
+   alpha_equiv_function_sig'_scheme vsubst fsubst n1 s1 n2 s2)"
 *)
+
+(* fun alpha_equiv_function_bodies' ::
+  "subst \<Rightarrow> ('g, 'v, 't) YulFunctionBody \<Rightarrow> ('g, 'v, 't) YulFunctionBody \<Rightarrow> bool" where
+(* TODO: see if we need it *)
+*)
+
+definition alpha_equiv_fun ::
+  "subst \<Rightarrow> subst \<Rightarrow> (YulIdentifier * ('g, 'v, 't) function_sig) \<Rightarrow> (YulIdentifier * ('g, 'v, 't) function_sig) \<Rightarrow> bool"
+  where
+"alpha_equiv_fun vsubst fsubst fun1 fun2 =
+  (case fun1 of (n1, s1) \<Rightarrow>
+  (case fun2 of (n2, s2) \<Rightarrow>
+  (alpha_equiv_function_sig'_scheme vsubst fsubst n1 s1 n2 s2)))"
 
 (* TODO: we aren't checking that types are compatible here. Perhaps this can be done
  * in a different pass *)
+(*
 fun alpha_equiv_funs' ::
-  "subst \<Rightarrow> ('g, 'v, 't) function_sig locals \<Rightarrow> ('g, 'v, 't) function_sig locals \<Rightarrow> bool"
+  "subst \<Rightarrow> subst \<Rightarrow> ('g, 'v, 't) function_sig locals \<Rightarrow> ('g, 'v, 't) function_sig locals \<Rightarrow> bool"
   where
-"alpha_equiv_funs' subst [] [] = True"
-| "alpha_equiv_funs' subst ((n1, s1)#t1) ((n2, s2)#t2) =
-   (alpha_equiv_function_sig' subst n1 s1 n2 s2 \<and>
-    alpha_equiv_funs' subst t1 t2)"
-| "alpha_equiv_funs' _ _ _ = False"
+"alpha_equiv_funs' vsubst fsubst [] [] = True"
+| "alpha_equiv_funs' vsubst fsubst ((n1, s1)#t1) ((n2, s2)#t2) =
+   (alpha_equiv_function_sig'_scheme vsubst fsubst n1 s1 n2 s2 \<and>
+    alpha_equiv_funs' vsubst fsubst t1 t2)"
+| "alpha_equiv_funs' _ _ _ _ = False"
+*)
+
+definition alpha_equiv_funs' ::
+  "subst \<Rightarrow> subst \<Rightarrow> ('g, 'v, 't) function_sig locals \<Rightarrow> ('g, 'v, 't) function_sig locals \<Rightarrow> bool"
+  where
+"alpha_equiv_funs' vsubst fsubst funs1 funs2 =
+  list_all2 (alpha_equiv_fun vsubst fsubst) funs1 funs2"
 
 (* TODO: make sure we are handling equivalence of function-contexts correctly.
  * this is a bit complicated to due to possibility of recursion/mutual recursion *)
 
 fun alpha_equiv_stackEl' ::
-  "subst \<Rightarrow> ('g, 'v, 't) StackEl \<Rightarrow> ('g, 'v, 't) StackEl \<Rightarrow> bool" where
-"alpha_equiv_stackEl' subst (EnterStatement s1) (EnterStatement s2) =
-  alpha_equiv_statement' subst s1 s2"
-| "alpha_equiv_stackEl' subst (ExitStatement s1 vs1 fs1) (ExitStatement s2 vs2 fs2) =
-    (alpha_equiv_statement' subst s1 s2 \<and>
-     alpha_equiv_locals' subst vs1 vs2 \<and>
-     alpha_equiv_funs' subst fs1 fs2)"
-| "alpha_equiv_stackEl' subst (Expression e1) (Expression e2) =
-  alpha_equiv_expr' subst e1 e2"
-| "alpha_equiv_stackEl' subst (EnterFunctionCall n1 f1) (EnterFunctionCall n2 f2) = 
-   (alpha_equiv_function_sig' subst n1 f1 n2 f2)"
-| "alpha_equiv_stackEl' subst (ExitFunctionCall n1 vals1 locals1 fs1 f1)
-                              (ExitFunctionCall n2 vals2 locals2 fs2 f2) =
-    (alpha_equiv_function_sig' subst n1 f1 n2 f2 \<and>
-     alpha_equiv_locals' subst locals1 locals2 \<and>
-     alpha_equiv_funs' subst fs1 fs2)"
-| "alpha_equiv_stackEl' subst _ _ = False"
+  "subst \<Rightarrow> subst \<Rightarrow> ('g, 'v, 't) StackEl \<Rightarrow> ('g, 'v, 't) StackEl \<Rightarrow> bool" where
+"alpha_equiv_stackEl' vsubst fsubst (EnterStatement s1) (EnterStatement s2) =
+  alpha_equiv_statement' vsubst fsubst s1 s2"
+| "alpha_equiv_stackEl' vsubst fsubst (ExitStatement s1 vs1 fs1) (ExitStatement s2 vs2 fs2) =
+    (alpha_equiv_statement' vsubst fsubst s1 s2 \<and>
+     alpha_equiv_locals' vsubst fsubst vs1 vs2 \<and>
+     alpha_equiv_funs' vsubst fsubst fs1 fs2)"
+| "alpha_equiv_stackEl' vsubst fsubst (Expression e1) (Expression e2) =
+  alpha_equiv_expr' vsubst fsubst e1 e2"
+| "alpha_equiv_stackEl' vsubst fsubst (EnterFunctionCall n1 f1) (EnterFunctionCall n2 f2) = 
+   (alpha_equiv_function_sig'_scheme vsubst fsubst n1 f1 n2 f2)"
+| "alpha_equiv_stackEl' vsubst fsubst (ExitFunctionCall n1 vals1 locals1 fs1 f1)
+                                      (ExitFunctionCall n2 vals2 locals2 fs2 f2) =
+    (alpha_equiv_function_sig'_scheme vsubst fsubst n1 f1 n2 f2 \<and>
+     alpha_equiv_locals' vsubst fsubst locals1 locals2 \<and>
+     alpha_equiv_funs' vsubst fsubst fs1 fs2)"
+| "alpha_equiv_stackEl' vsubst fsubst _ _ = False"
 
 (* whenever we extend the variable context, we also need to update subst.  *)
 (* also need to update subst on function entry. *)
@@ -322,13 +358,13 @@ fun alpha_equiv_stackEl' ::
 (* gather yul functions / get_fun_decls *)
 
 fun subst_update_enter_statement ::
-  "subst \<Rightarrow>
+  "subst \<Rightarrow> subst \<Rightarrow>
    ('v, 't) YulStatement \<Rightarrow>
    ('v, 't) YulStatement \<Rightarrow>
-   subst" where
-"subst_update_enter_statement subst (YulBlock ls1) (YulBlock ls2) =
-  (zip (get_fun_decls ls1) (get_fun_decls ls2))# subst"
-| "subst_update_enter_statement subst _ _ = subst"
+   (subst * subst)" where
+"subst_update_enter_statement vsubst fsubst (YulBlock ls1) (YulBlock ls2) =
+  (vsubst, (zip (get_fun_decls ls1) (get_fun_decls ls2))# fsubst)"
+| "subst_update_enter_statement vsubst fsubst _ _ = (vsubst, fsubst)"
 
 (*
 fun YulStatement_same_constr ::
@@ -337,64 +373,551 @@ fun YulStatement_same_constr ::
 | "YulStatement_same_constr _ _ = False"
 *)
 fun subst_update_exit_statement ::
-  "subst \<Rightarrow>
+  "subst \<Rightarrow> subst \<Rightarrow>
    ('v, 't) YulStatement \<Rightarrow>
    ('v, 't) YulStatement \<Rightarrow>
-   subst option" where
-"subst_update_exit_statement subst
+   (subst * subst) option" where
+"subst_update_exit_statement vsubst fsubst
   (YulVariableDeclarationStatement (YulVariableDeclaration ns1 eo1))
   (YulVariableDeclarationStatement (YulVariableDeclaration ns2 eo2)) = 
-  (case subst of
-    sh # subst \<Rightarrow> Some ((sh @ (zip (strip_id_types ns1) (strip_id_types ns2))) # subst)
+  (case vsubst of
+    sh # subst \<Rightarrow>
+      Some ((((zip (strip_id_types ns1) (strip_id_types ns2)) @ sh) # subst), fsubst)
     | _ \<Rightarrow> None)"
-| "subst_update_exit_statement subst
+| "subst_update_exit_statement vsubst fsubst
   (YulBlock ls1)
   (YulBlock ls2) = 
-  (case subst of
-    sh # subst \<Rightarrow> Some subst
+  (case (vsubst, fsubst) of
+    (vsh # vsubst', fsh # fsubst') \<Rightarrow> Some (vsubst', fsubst')
    | _ \<Rightarrow> None)"
-| "subst_update_exit_statement subst _ _ = Some subst" (* bogus cases mixed with noop cases here. *)
+(* bogus cases mixed with noop cases here. *)
+| "subst_update_exit_statement vsubst fsubst _ _ = Some (vsubst, fsubst)" 
 
-(* TODO: figure out if we need to change
-   yul_statement_to_deBruijn to separate the function define/return scope
-   from the scope of the function local variables (declared inside a block)
-
-   maybe this doesn't matter though. the subst we generate will
-   still be valid, even if it isn't the one generated by
-   the renamer?
- *)
 fun subst_update_enter_fun_call ::
-    "subst \<Rightarrow> ('g, 'v, 't) function_sig \<Rightarrow> ('g, 'v, 't) function_sig \<Rightarrow> subst"
+    "subst \<Rightarrow> subst \<Rightarrow> ('g, 'v, 't) function_sig \<Rightarrow> ('g, 'v, 't) function_sig \<Rightarrow> (subst * subst)"
     where
-  "subst_update_enter_fun_call subst 
+  "subst_update_enter_fun_call vsubst fsubst
     sig1 sig2 = 
     (case (f_sig_body sig1, f_sig_body sig2) of
       (YulFunction b1, YulFunction b2) \<Rightarrow>
-        (zip ((map (\<lambda> x . case x of (YulTypedName n t) \<Rightarrow> n) (f_sig_arguments sig1)) @
-             (map (\<lambda> x . case x of (YulTypedName n t) \<Rightarrow> n) (f_sig_returns sig1)))
-             ((map (\<lambda> x . case x of (YulTypedName n t) \<Rightarrow> n) (f_sig_arguments sig2)) @
-             (map (\<lambda> x . case x of (YulTypedName n t) \<Rightarrow> n) (f_sig_returns sig1)))) # subst
-      | (_, _) \<Rightarrow> subst)
+        ((zip ((map (\<lambda> x . case x of (YulTypedName n t) \<Rightarrow> n) (f_sig_arguments sig1)) @
+              (map (\<lambda> x . case x of (YulTypedName n t) \<Rightarrow> n) (f_sig_returns sig1)))
+              ((map (\<lambda> x . case x of (YulTypedName n t) \<Rightarrow> n) (f_sig_arguments sig2)) @
+              (map (\<lambda> x . case x of (YulTypedName n t) \<Rightarrow> n) (f_sig_returns sig1)))) # vsubst
+        , fsubst)
+      | (_, _) \<Rightarrow> (vsubst, fsubst))
     "
 
 fun subst_update_exit_fun_call ::
-  "subst \<Rightarrow> subst option"
+  "subst \<Rightarrow> subst \<Rightarrow> (subst * subst) option"
   where
-"subst_update_exit_fun_call (sh#subst) = Some subst"
-| "subst_update_exit_fun_call subst = None"
+"subst_update_exit_fun_call (vh#vsubst') (fsh # fsubst') = Some (vsubst', fsubst')"
+| "subst_update_exit_fun_call vsubst fsubst = None"
 
 (* TODO: return an option? *)
 fun subst_update ::
-  "subst \<Rightarrow> ('g, 'v, 't) StackEl \<Rightarrow> ('g, 'v, 't) StackEl \<Rightarrow> subst option" where
-"subst_update subst (EnterStatement s1) (EnterStatement s2) =
-  Some (subst_update_enter_statement subst s1 s2)"
-| "subst_update subst (ExitStatement s1 _ _) (ExitStatement s2 _ _) =
-  subst_update_exit_statement subst s1 s2"
-| "subst_update subst (EnterFunctionCall f1 s1) (EnterFunctionCall f2 s2) =
-  Some (subst_update_enter_fun_call subst s1 s2)"
-| "subst_update subst (ExitFunctionCall _ _ _ _ _) (ExitFunctionCall _ _ _ _ _) = 
-  subst_update_exit_fun_call subst"
-| "subst_update subst _ _ = Some subst"
+  "subst \<Rightarrow> subst \<Rightarrow> ('g, 'v, 't) StackEl \<Rightarrow> ('g, 'v, 't) StackEl \<Rightarrow> (subst * subst) option" where
+"subst_update vsubst fsubst (EnterStatement s1) (EnterStatement s2) =
+  Some (subst_update_enter_statement vsubst fsubst s1 s2)"
+| "subst_update vsubst fsubst (ExitStatement s1 _ _) (ExitStatement s2 _ _) =
+  subst_update_exit_statement vsubst fsubst s1 s2"
+| "subst_update vsubst fsubst (EnterFunctionCall f1 s1) (EnterFunctionCall f2 s2) =
+  Some (subst_update_enter_fun_call vsubst fsubst s1 s2)"
+| "subst_update vsubst fsubst (ExitFunctionCall _ _ _ _ _) (ExitFunctionCall _ _ _ _ _) = 
+  subst_update_exit_fun_call vsubst fsubst"
+| "subst_update vsubst fsubst _ _ = Some (vsubst, fsubst)"
+
+definition alpha_equiv_results' ::
+  "subst \<Rightarrow> subst \<Rightarrow>
+   ('g, 'v, 't) YulInput \<Rightarrow>
+   ('g, 'v, 't) YulInput \<Rightarrow>
+   bool" where
+"alpha_equiv_results' vsubst fsubst r1 r2 =
+  (global r1 = global r2 \<and>
+   vals r1 = vals r2 \<and>
+   alpha_equiv_locals' vsubst fsubst (locals r1) (locals r2) \<and>
+   alpha_equiv_funs' vsubst fsubst (funs r1) (funs r2) \<and>
+   (list_all2 (alpha_equiv_stackEl' vsubst fsubst)
+              (cont r1)
+              (cont r2)))"
+
+lemma alpha_equiv_locals'_length :
+  assumes "alpha_equiv_locals' vsubst fsubst l1 l2"
+  shows "length l1 = length l2"
+  using assms
+proof(induction l1 arbitrary: vsubst fsubst l2)
+  case Nil
+  then show ?case 
+    by(cases l2; auto simp add: alpha_equiv_locals'_def)
+next
+  case (Cons l1h l1t)
+
+  show ?case
+  proof(cases l2)
+    case Nil' : Nil
+    then show ?thesis using Cons
+      by(auto simp add: alpha_equiv_locals'_def)
+  next
+    case Cons' : (Cons l2h l2t)
+    then show ?thesis using Cons.prems Cons.IH[of vsubst fsubst l2t]
+      by(cases l1h; cases l2h; auto simp add: alpha_equiv_locals'_def)
+  qed
+qed
+
+lemma alpha_equiv_locals_v_insert1_unmentioned :
+  assumes "alpha_equiv_locals' (vsubsth # vsubstt) fsubst l1 l2"
+  assumes "map_of l1 n1 = None"
+  assumes "map_of l2 n2 = None" 
+  shows "alpha_equiv_locals' (((n1, n2) # vsubsth) # vsubstt) fsubst l1 l2"
+  using assms
+proof(induction l1 arbitrary: vsubsth vsubstt l2 n1 n2)
+  case Nil
+  then show ?case
+    by(cases l2; auto simp add: alpha_equiv_locals'_def)
+next
+  case (Cons l1h l1t)
+
+  obtain l2h l2t where Cons2 :
+    "l2 = l2h # l2t"
+    using Cons.prems
+    by(cases l2; auto simp add: alpha_equiv_locals'_def)
+
+  show ?case 
+    using Cons.prems Cons.IH[of vsubsth vsubstt l2t n1 n2] Cons2
+    by(cases l1h; cases l2h; auto simp add: alpha_equiv_locals'_def alpha_equiv_local_def split: option.splits if_splits)
+qed
+
+(* NB: induction not needed here. *)
+lemma alpha_equiv_locals_v_insert1 :
+  assumes H1 : "insert_value l1 n1 v = Some l1'"
+  assumes H2 : "insert_value l2 n2 v = Some l2'"
+  assumes "alpha_equiv_locals' (vsubsth # vsubstt) fsubst l1 l2"
+  shows "alpha_equiv_locals' (((n1, n2)#vsubsth) # vsubstt) fsubst l1' l2'"
+  using assms
+proof(induction vsubstt arbitrary: vsubsth n1 n2 v l1 l2 l1' l2')
+  case Nil
+  then show ?case using alpha_equiv_locals_v_insert1_unmentioned[of vsubsth "[]" fsubst l1 l2]
+    by(auto simp add: alpha_equiv_locals'_def alpha_equiv_local_def split: option.splits)
+next
+  case (Cons vsubsth' vsubstt')
+  show ?case using Cons.prems
+    alpha_equiv_locals_v_insert1_unmentioned[of vsubsth "vsubsth' # vsubstt'" fsubst l1 l2 n1 n2]
+    using Cons.prems
+    by(auto simp add: alpha_equiv_locals'_def alpha_equiv_local_def split: option.splits)
+qed
+
+
+lemma alpha_equiv_locals_v_insert :
+  assumes H1 : "insert_values l1 ns1 vs = Some l1'"
+  assumes H2 : "insert_values l2 ns2 vs = Some l2'"
+  assumes "alpha_equiv_locals' (vsubsth # vsubstt) fsubst l1 l2"
+  shows "alpha_equiv_locals' ((zip ns1 ns2 @ vsubsth) # vsubstt) fsubst l1' l2'"
+  using assms
+proof(induction vs arbitrary: vsubsth vsubstt ns1 ns2 l1 l2 l1' l2')
+  case Nil
+
+  have Nil1 : "ns1 = []"
+    using Nil
+    by(cases ns1; auto)
+
+  have Nil2 : "ns2 = []"
+    using Nil
+    by(cases ns2; auto)
+
+  show ?case using Nil Nil1 Nil2
+    by(auto)
+next
+  case (Cons vh vt)
+
+  obtain n1h n1t where Cons1 : "ns1 = n1h#n1t"
+    using Cons
+    by(cases ns1; auto)
+
+  obtain n2h n2t where Cons2 : "ns2 = n2h#n2t"
+    using Cons
+    by(cases ns2; auto)
+
+  obtain l1't where L1't : "insert_values l1 n1t vt = Some l1't" "insert_value l1't n1h vh = Some l1'"
+    using Cons1 Cons.prems
+    by(auto split: option.split_asm)
+
+  obtain l2't where L2't : "insert_values l2 n2t vt = Some l2't" "insert_value l2't n2h vh = Some l2'"
+    using Cons2 Cons.prems
+    by(auto split: option.split_asm)
+
+  have Conc' : "alpha_equiv_locals' ((zip n1t n2t @ vsubsth) # vsubstt) fsubst l1't l2't"
+    using Cons1 Cons2 Cons.IH[OF L1't(1) L2't(1) Cons.prems(3)]
+    by(auto)
+
+  show ?case
+    using alpha_equiv_locals_v_insert1[OF L1't(2) L2't(2) Conc'] Cons1 Cons2
+    by(auto)
+qed
+
+(* TODO: do we need an additional assumption that locals and funs
+ * don't have name collisions?
+ *)
+(*
+lemma alpha_equiv_function_sig'_insert1_unmentioned :
+  assumes "alpha_equiv_function_sig' (substh # substt) l1 l2"
+  assumes "map_of l1 n1 = None"
+  assumes "map_of l2 n2 = None" 
+  shows "alpha_equiv_function_sig' (((n1, n2) # substh) # substt) l1 l2"
+  using assms
+proof(induction l1 arbitrary: substh substt l2 n1 n2)
+  case Nil
+  then show ?case
+    by(cases l2; auto)
+next
+  case (Cons l1h l1t)
+
+  obtain l2h l2t where Cons2 :
+    "l2 = l2h # l2t"
+    using Cons.prems
+    by(cases l2; auto)
+
+  show ?case 
+    using Cons.prems Cons.IH[of substh substt l2t n1 n2] Cons2
+    apply(cases l1h; cases l2h; auto split: if_splits)
+    apply( simp add: alpha_equiv_function_sig'_def split: option.splits if_splits)
+qed
 *)
+
+(* make sure builtins are mentioned in subst? *)
+(* problem: need to recurse into functions in order to see if
+ * there is a name collision... *)
+lemma alpha_equiv_funs_f_insert1_unmentioned :
+  assumes "alpha_equiv_funs' vsubst (fsubsth # fsubstt) l1 l2"
+  assumes "map_of l1 n1 = None"
+  assumes "map_of l2 n2 = None" 
+  shows "alpha_equiv_funs' vsubst (((n1, n2) # fsubsth) # fsubstt) l1 l2"
+  using assms
+proof(induction l1 arbitrary: vsubst fsubsth fsubstt l2 n1 n2)
+  case Nil
+  then show ?case
+    by(cases l2; auto simp add: alpha_equiv_funs'_def)
+next
+  case (Cons l1h l1t)
+
+  obtain l2h l2t where Cons2 :
+    "l2 = l2h # l2t"
+    using Cons.prems
+    by(cases l2; auto simp add: alpha_equiv_funs'_def)
+
+  show ?case 
+    using Cons.prems Cons.IH[of vsubst fsubsth fsubstt l2t n1 n2] Cons2
+    unfolding alpha_equiv_funs'_def alpha_equiv_fun_def
+    apply(cases l1h; cases l2h; auto split: if_splits)
+    apply(auto simp add:  alpha_equiv_function_sig'_scheme_def
+          alpha_equiv_name'_def split: option.splits if_splits YulFunctionBody.splits)
+qed
+
+
+lemma alpha_equiv_funs_f_insert1 :
+  assumes H1 : "insert_value l1 n1 v = Some l1'"
+  assumes H2 : "insert_value l2 n2 v = Some l2'"
+  assumes "alpha_equiv_funs' (substh # substt) l1 l2"
+  shows "alpha_equiv_funs' (((n1, n2)#substh) # substt) l1' l2'"
+  using assms
+proof(induction substt arbitrary: substh n1 n2 v l1 l2 l1' l2')
+  case Nil
+  then show ?case using alpha_equiv_locals_insert1_unmentioned[of substh "[]" l1 l2]
+    by(auto split: option.splits)
+next
+  case (Cons substh' substt')
+  show ?case using Cons.prems
+    alpha_equiv_locals_insert1_unmentioned[of substh "substh' # substt'" l1 l2 n1 n2]
+    using Cons.prems
+    by(auto split: option.splits)
+qed
+
+
+lemma alpha_equiv_funs_insert :
+  assumes H1 : "insert_values l1 ns1 vs = Some l1'"
+  assumes H2 : "insert_values l2 ns2 vs = Some l2'"
+  assumes "alpha_equiv_funs' (substh # substt) l1 l2"
+  shows "alpha_equiv_funs' ((zip ns1 ns2 @ substh) # substt) l1' l2'"
+  using assms
+proof(induction vs arbitrary: substh substt ns1 ns2 l1 l2 l1' l2')
+  case Nil
+
+  have Nil1 : "ns1 = []"
+    using Nil
+    by(cases ns1; auto)
+
+  have Nil2 : "ns2 = []"
+    using Nil
+    by(cases ns2; auto)
+
+  show ?case using Nil Nil1 Nil2
+    by(auto)
+next
+  case (Cons vh vt)
+
+  obtain n1h n1t where Cons1 : "ns1 = n1h#n1t"
+    using Cons
+    by(cases ns1; auto)
+
+  obtain n2h n2t where Cons2 : "ns2 = n2h#n2t"
+    using Cons
+    by(cases ns2; auto)
+
+  obtain l1't where L1't : "insert_values l1 n1t vt = Some l1't" "insert_value l1't n1h vh = Some l1'"
+    using Cons1 Cons.prems
+    by(auto split: option.split_asm)
+
+  obtain l2't where L2't : "insert_values l2 n2t vt = Some l2't" "insert_value l2't n2h vh = Some l2'"
+    using Cons2 Cons.prems
+    by(auto split: option.split_asm)
+
+  have Conc' : "alpha_equiv_funs' ((zip n1t n2t @ substh) # substt) l1't l2't"
+    using Cons1 Cons2 Cons.IH[OF L1't(1) L2't(1) Cons.prems(3)]
+    by(auto)
+
+  show ?case
+    using alpha_equiv_insert1[OF L1't(2) L2't(2) Conc'] Cons1 Cons2
+    by(auto)
+qed
+
+(* need a lemma about alpha_equiv_stackEl'
+ * and consing onto the front of the vars/funs lists.
+ *)
+
+lemma alpha_equiv_step :
+  assumes Hc1 : "cont r1 = (c1h#c1t)"
+  assumes Hc2 : "cont r2 = (c2h#c2t)"
+  assumes Hinit : "alpha_equiv_results' vsubst fsubst r1 r2"
+  assumes H1 : "evalYulStep d r1 = YulResult r1'"
+  assumes H2 : "evalYulStep d r2 = YulResult r2'"
+  assumes Hupd : "subst_update vsubst fsubst c1h c2h = Some (vsubst', fsubst')"
+  shows "alpha_equiv_results' vsubst' fsubst' r1' r2'"
+  using assms
+proof(cases c1h)
+  case ES1 : (EnterStatement x1)
+
+  then obtain x2 where ES2 : "c2h = EnterStatement x2"
+    using Hc1 Hc2 Hinit
+    by(cases c2h; auto simp add: alpha_equiv_results'_def)
+
+  show ?thesis
+  proof(cases x1)
+    case F1: (YulFunctionCallStatement f1)
+
+    then obtain n1 args1 where 
+      FC1 : "f1 = YulFunctionCall n1 args1"
+      by(cases f1; auto)
+
+    obtain f2 where F2 :
+      "x2 = YulFunctionCallStatement f2"
+      using ES1 ES2 F1 FC1 Hc1 Hc2 Hinit
+      by(cases x2; auto simp add: alpha_equiv_results'_def)
+
+    then obtain n2 args2 where
+      FC2 : "f2 = YulFunctionCall n2 args2"
+      by(cases f2; auto)
+
+    show ?thesis 
+      using ES1 F1 FC1 ES2 F2 FC2 Hinit H1 H2 Hc1 Hc2 Hupd
+      by(auto simp add: alpha_equiv_results'_def)
+  next
+
+    case A1 : (YulAssignmentStatement a1)
+
+    then obtain vs1 e1 where
+      AS1 : "a1 = YulAssignment vs1 e1"
+      by(cases a1; auto)
+
+    obtain a2 where A2 :
+      "x2 = YulAssignmentStatement a2"
+      using ES1 ES2 A1 AS1 Hc1 Hc2 Hinit
+      by(cases x2; auto simp add: alpha_equiv_results'_def)
+
+    then obtain vs2 e2 where
+      AS2 : "a2 = YulAssignment vs2 e2"
+      by(cases a2; auto)
+
+    show ?thesis
+      using ES1 A1 AS1 ES2 A2 AS2 Hinit H1 H2 Hc1 Hc2 Hupd
+      by(auto simp add: alpha_equiv_results'_def)
+  next
+    case D1 : (YulVariableDeclarationStatement d1)
+
+    then obtain vs1 eo1 where
+      VD1 : "d1 = YulVariableDeclaration vs1 eo1"
+      by(cases d1; auto)
+
+    obtain d2 where
+      D2 : "x2 = YulVariableDeclarationStatement d2"
+      using ES1 ES2 D1 VD1 Hc1 Hc2 Hinit
+      by(cases x2; auto simp add: alpha_equiv_results'_def)
+
+    then obtain vs2 eo2 where
+      VD2 : "d2 = YulVariableDeclaration vs2 eo2"
+      by(cases d2; auto)
+
+    show ?thesis
+      using ES1 D1 VD1 ES2 D2 VD2 Hinit H1 H2 Hc1 Hc2 Hupd
+      by(cases eo1; cases eo2; auto simp add: alpha_equiv_results'_def)
+  next
+    case (YulFunctionDefinitionStatement x4)
+    then show ?thesis sorry
+  next
+    case (YulIf x51 x52)
+    then show ?thesis sorry
+  next
+  case (YulSwitch x61 x62)
+    then show ?thesis sorry
+  next
+    case (YulForLoop x71 x72 x73 x74)
+    then show ?thesis sorry
+  next
+    case YulBreak
+    then show ?thesis sorry
+  next
+    case YulContinue
+    then show ?thesis sorry
+  next
+    case YulLeave
+    then show ?thesis sorry
+  next
+    case (YulBlock x11)
+    then show ?thesis sorry
+  qed
+
+next
+  case XS1 : (ExitStatement x1 locs1 funs1)
+
+  then obtain x2 locs2 funs2 where XS2 : "c2h = ExitStatement x2 locs2 funs2"
+    using Hc1 Hc2 Hinit
+    by(cases c2h; auto simp add: alpha_equiv_results'_def)
+
+  show ?thesis
+  proof(cases x1)
+    case F1 : (YulFunctionCallStatement f1)
+
+    then obtain n1 args1 where 
+      FC1 : "f1 = YulFunctionCall n1 args1"
+      by(cases f1; auto)
+
+    obtain f2 where F2 :
+      "x2 = YulFunctionCallStatement f2"
+      using XS1 XS2 F1 FC1 Hc1 Hc2 Hinit
+      by(cases x2; auto simp add: alpha_equiv_results'_def)
+
+    then obtain n2 args2 where
+      FC2 : "f2 = YulFunctionCall n2 args2"
+      by(cases f2; auto)
+
+    show ?thesis 
+      using XS1 F1 FC1 XS2 F2 FC2 Hinit H1 H2 Hc1 Hc2 Hupd
+      by(cases "vals r2"; auto simp add: alpha_equiv_results'_def)
+
+  next
+    case (YulAssignmentStatement x2)
+    then show ?thesis sorry
+  next
+    case D1 : (YulVariableDeclarationStatement d1)
+
+    then obtain vs1 eo1 where
+      VD1 : "d1 = YulVariableDeclaration vs1 eo1"
+      by(cases d1; auto)
+
+    obtain d2 where
+      D2 : "x2 = YulVariableDeclarationStatement d2"
+      using XS1 XS2 D1 VD1 Hc1 Hc2 Hinit
+      by(cases x2; auto simp add: alpha_equiv_results'_def)
+
+    then obtain vs2 eo2 where
+      VD2 : "d2 = YulVariableDeclaration vs2 eo2"
+      by(cases d2; auto)
+
+    show ?thesis
+    proof(cases eo1)
+      case None1 : None
+
+      then have None2 : "eo2 = None"
+        using XS1 D1 VD1 XS2 D2 VD2 Hinit H1 H2 Hc1 Hc2 Hupd
+        by(cases eo2; auto simp add: alpha_equiv_results'_def)
+
+      have Vemp : "vals r1 = []" 
+        using XS1 D1 VD1 XS2 D2 VD2 Hinit H1 H2 Hc1 Hc2 Hupd None1 None2
+        by(cases "vals r2"; auto simp add: alpha_equiv_results'_def)
+
+      obtain substh substt where Subst_cons :
+        "vsubst = substh#substt"
+        using XS1 D1 VD1 XS2 D2 VD2 Hinit H1 H2 Hc1 Hc2 Hupd None1 None2 Vemp
+        by(cases vsubst; auto simp add: alpha_equiv_results'_def)
+
+      obtain L1 where L1v :
+        "insert_values (locals r1) (map strip_id_type vs1) (replicate (length vs1) (default_val d)) = Some L1"
+        using XS1 D1 VD1 XS2 D2 VD2 Hinit H1 H2 Hc1 Hc2 Hupd None1 None2 Vemp Subst_cons
+        by(auto simp add: alpha_equiv_results'_def split: option.split_asm)
+
+      obtain L2 where L2v :
+        "insert_values (locals r2) (map strip_id_type vs2) (replicate (length vs2) (default_val d)) = Some L2"
+        using XS1 D1 VD1 XS2 D2 VD2 Hinit H1 H2 Hc1 Hc2 Hupd None1 None2 Vemp Subst_cons
+        by(auto simp add: alpha_equiv_results'_def split: option.split_asm)
+
+      have Vlens : "length vs1 = length vs2"
+        using XS1 D1 VD1 XS2 D2 VD2 Hinit H1 H2 Hc1 Hc2 
+        by(auto simp add: alpha_equiv_results'_def)
+
+      show ?thesis using XS1 D1 VD1 XS2 D2 VD2 Hinit H1 H2 Hc1 Hc2 Hupd None1 None2 Vemp Subst_cons
+          L1v L2v
+          alpha_equiv_locals_v_insert[OF L1v[unfolded Vlens] L2v, of substh substt fsubst']
+        apply(auto simp add: alpha_equiv_results'_def)
+          defer
+
+    next
+      case (Some a)
+      then show ?thesis sorry
+    qed
+
+
+      using XS1 D1 VD1 XS2 D2 VD2 Hinit H1 H2 Hc1 Hc2 Hupd
+      apply(cases eo1; cases eo2; auto simp add: alpha_equiv_results'_def)
+(* again, we need a lemma relating updates to alpha-equivalence *)
+  next
+
+    case (YulVariableDeclarationStatement x3)
+    then show ?thesis sorry
+  next
+    case (YulFunctionDefinitionStatement x4)
+    then show ?thesis sorry
+  next
+  case (YulIf x51 x52)
+  then show ?thesis sorry
+  next
+    case (YulSwitch x61 x62)
+    then show ?thesis sorry
+  next
+    case (YulForLoop x71 x72 x73 x74)
+    then show ?thesis sorry
+  next
+    case YulBreak
+    then show ?thesis sorry
+  next
+    case YulContinue
+    then show ?thesis sorry
+  next
+    case YulLeave
+    then show ?thesis sorry
+  next
+    case (YulBlock x11)
+    then show ?thesis sorry
+  qed
+
+  then show ?thesis sorry
+next
+  case (EnterFunctionCall x31 x32)
+  then show ?thesis sorry
+next
+  case (ExitFunctionCall x41 x42 x43 x44 x45)
+  then show ?thesis sorry
+next
+  case (Expression x5)
+  then show ?thesis sorry
+qed
+
 
 end
